

# Quantum Tunneling through a Single Potential Barrier: An Analytical Approach

Rati Kaewkam

9 November 2025

## Problem Setup

Suppose the potential  $V(x)$  is given by:

$$V(x) = \begin{cases} V_0, & 0 \leq x \leq L \\ 0, & \text{otherwise} \end{cases}$$

We analyze the case for a particle with energy  $E > 0$  incident from the left. This paper focuses on the quantum tunneling, so we assume the particle's energy is less than the barrier height:  $0 < E < V_0$ .

## Time-independent Schrödinger equation

$$-\frac{\hbar^2}{2m} \frac{d^2\psi}{dx^2} + V\psi = E\psi$$

## Wave Function Solutions in Each Region

**Region I** ( $x < 0, V = 0$ )

$$-\frac{\hbar^2}{2m} \frac{d^2\psi_I}{dx^2} = E\psi_I \implies \frac{d^2\psi_I}{dx^2} + k_1^2\psi_I = 0$$

Define  $k_1^2 = \frac{2mE}{\hbar^2}$

$$\psi_I(x) = Ae^{ik_1x} + Be^{-ik_1x}$$

**Region II** ( $0 \leq x \leq L, V = V_0$ )

$$-\frac{\hbar^2}{2m} \frac{d^2\psi_{II}}{dx^2} + V_0\psi_{II} = E\psi_{II} \implies \frac{d^2\psi_{II}}{dx^2} - k_2^2\psi_{II} = 0$$

Define  $k_2^2 = \frac{2m(V_0-E)}{\hbar^2}$

$$\psi_{II}(x) = Ce^{k_2x} + De^{-k_2x}$$

**Region III** ( $x > L, V = 0$ )

$$-\frac{\hbar^2}{2m} \frac{d^2 \psi_{III}}{dx^2} = E \psi_{III} \implies \frac{d^2 \psi_{III}}{dx^2} + k_1^2 \psi_{III} = 0$$

Define  $k_1^2 = \frac{2mE}{\hbar^2}$

$$\psi_{III}(x) = F e^{ik_1 x}$$

## From the boundary conditions

We apply continuity for  $\psi(x)$  and  $\frac{d\psi}{dx}$  at both  $x = 0$  and  $x = L$ . This gives four conditions:

$$\psi_I(0) = \psi_{II}(0) \implies A + B = C + D \quad (1)$$

$$\psi_{II}(L) = \psi_{III}(L) \implies C e^{k_2 L} + D e^{-k_2 L} = F e^{ik_1 L} \quad (2)$$

$$\left. \frac{d\psi_I}{dx} \right|_{x=0} = \left. \frac{d\psi_{II}}{dx} \right|_{x=0} \implies ik_1(A - B) = k_2(C - D) \quad (3)$$

$$\left. \frac{d\psi_{II}}{dx} \right|_{x=L} = \left. \frac{d\psi_{III}}{dx} \right|_{x=L} \implies k_2(C e^{k_2 L} - D e^{-k_2 L}) = ik_1 F e^{ik_1 L} \quad (4)$$

## Solving the system

From (2) and (4):

$$(2) + \frac{(4)}{k_2} \implies 2C e^{k_2 L} = \left(1 + \frac{ik_1}{k_2}\right) F e^{ik_1 L}$$

$$C = \left(1 + \frac{ik_1}{k_2}\right) \frac{F}{2} e^{ik_1 L - k_2 L} \quad (5)$$

$$(2) - \frac{(4)}{k_2} \implies 2D e^{-k_2 L} = \left(1 - \frac{ik_1}{k_2}\right) F e^{ik_1 L}$$

$$D = \left(1 - \frac{ik_1}{k_2}\right) \frac{F}{2} e^{ik_1 L + k_2 L} \quad (6)$$

From (1) and (3):

$$(1) + \frac{(3)}{ik_1} \implies 2A = \left(1 - \frac{ik_2}{k_1}\right) C + \left(1 + \frac{ik_2}{k_1}\right) D \quad (7)$$

Note: Define  $\gamma = \frac{k_1^2 - k_2^2}{k_1 k_2}$ . Then:

$$\left(1 - \frac{ik_2}{k_1}\right) \left(1 + \frac{ik_1}{k_2}\right) = 2 + i \left(\frac{k_1^2 - k_2^2}{k_1 k_2}\right) = 2 + i\gamma$$

$$\left(1 + \frac{ik_2}{k_1}\right) \left(1 - \frac{ik_1}{k_2}\right) = 2 - i \left(\frac{k_1^2 - k_2^2}{k_1 k_2}\right) = 2 - i\gamma$$

Substitute (5) and (6) into the equation for  $2A$  (eq. 7):

$$\begin{aligned}
2A &= \left[ \left(1 - \frac{ik_2}{k_1}\right) \left(1 + \frac{ik_1}{k_2}\right) \frac{F}{2} e^{ik_1 L - k_2 L} + \left(1 + \frac{ik_2}{k_1}\right) \left(1 - \frac{ik_1}{k_2}\right) \frac{F}{2} e^{ik_1 L + k_2 L} \right] \\
2A &= \frac{F}{2} e^{ik_1 L} [(2 + i\gamma)e^{-k_2 L} + (2 - i\gamma)e^{k_2 L}] \\
2A &= \frac{F}{2} e^{ik_1 L} [2(e^{k_2 L} + e^{-k_2 L}) - i\gamma(e^{k_2 L} - e^{-k_2 L})] \\
2A &= F e^{ik_1 L} [2 \cosh(k_2 L) - i\gamma \sinh(k_2 L)]
\end{aligned}$$

Now, we find the transmission amplitude  $\frac{F}{A}$ :

$$\frac{F}{A} = \frac{2e^{-ik_1 L}}{2 \cosh(k_2 L) - i\gamma \sinh(k_2 L)} = \frac{e^{-ik_1 L}}{\cosh(k_2 L) - \frac{i\gamma}{2} \sinh(k_2 L)}$$

The Transmission Probability:  $T = \left| \frac{F}{A} \right|^2 = \left( \frac{F}{A} \right) \left( \frac{F}{A} \right)^*$

$$\begin{aligned}
T &= \left( \frac{e^{-ik_1 L}}{\cosh(k_2 L) - \frac{i\gamma}{2} \sinh(k_2 L)} \right) \left( \frac{e^{+ik_1 L}}{\cosh(k_2 L) + \frac{i\gamma}{2} \sinh(k_2 L)} \right) \\
T &= \frac{1}{\cosh^2(k_2 L) + \left(\frac{\gamma}{2}\right)^2 \sinh^2(k_2 L)}
\end{aligned}$$

## Approximation for $k_2 L \gg 1$

If  $k_2 L \gg 1$ , then  $\cosh(k_2 L) \approx \frac{e^{k_2 L}}{2}$  and  $\sinh(k_2 L) \approx \frac{e^{k_2 L}}{2}$ . The denominator becomes:

$$\cosh^2(k_2 L) + \left(\frac{\gamma}{2}\right)^2 \sinh^2(k_2 L) \approx \left(\frac{e^{k_2 L}}{2}\right)^2 + \left(\frac{\gamma}{2}\right)^2 \left(\frac{e^{k_2 L}}{2}\right)^2 = \frac{e^{2k_2 L}}{4} \left(1 + \frac{\gamma^2}{4}\right)$$

So,

$$T \approx \frac{1}{\frac{e^{2k_2 L}}{4} \left(1 + \frac{\gamma^2}{4}\right)} = \frac{4e^{-2k_2 L}}{1 + \frac{\gamma^2}{4}}$$

We simplify the  $1 + \frac{\gamma^2}{4}$  term:

$$\begin{aligned}
1 + \frac{\gamma^2}{4} &= 1 + \frac{1}{4} \left( \frac{k_1^2 - k_2^2}{k_1 k_2} \right)^2 = \frac{4k_1^2 k_2^2 + (k_1^2 - k_2^2)^2}{4k_1^2 k_2^2} \\
&= \frac{4k_1^2 k_2^2 + k_1^4 - 2k_1^2 k_2^2 + k_2^4}{4k_1^2 k_2^2} = \frac{(k_1^2 + k_2^2)^2}{4k_1^2 k_2^2}
\end{aligned}$$

Substitute  $k_1^2 = \frac{2mE}{\hbar^2}$  and  $k_2^2 = \frac{2m(V_0-E)}{\hbar^2}$ :

$$\begin{aligned} k_1^2 + k_2^2 &= \frac{2mV_0}{\hbar^2} \\ 4k_1^2 k_2^2 &= 4 \left( \frac{2mE}{\hbar^2} \right) \left( \frac{2m(V_0-E)}{\hbar^2} \right) \\ 1 + \frac{\gamma^2}{4} &= \frac{\left( \frac{2mV_0}{\hbar^2} \right)^2}{4 \left( \frac{2mE}{\hbar^2} \right) \left( \frac{2m(V_0-E)}{\hbar^2} \right)} = \frac{V_0^2}{4E(V_0-E)} \end{aligned}$$

Finally, substituting this back into the expression for  $T$ :

$$\begin{aligned} T &\approx \frac{4e^{-2k_2L}}{\frac{V_0^2}{4E(V_0-E)}} = \frac{16E(V_0-E)}{V_0^2} e^{-2k_2L} \\ T &\approx \frac{16E}{V_0} \left( 1 - \frac{E}{V_0} \right) e^{-2k_2L} \end{aligned}$$